src/SchemaWellFormedness.v
@@ -58,28 +58,31 @@ Section WellFormedness.
       Subtype sch ty ty' ->
       Subtype sch (ListType ty) (ListType ty'). 
 
-  Fixpoint is_subtype sch (ty ty' : type) : bool :=
-    match ty, ty' with
-    | (ListType lty), (ListType lty') => is_subtype sch lty lty'
-    | (NT name), (NT name') => [|| (name == name'),
-                               declares_implementation sch ty ty' | 
-                              (name \in (union_members sch name'))]
-    | _, _ => false
-    end.
+  Equations is_subtype sch (ty ty' : @type Name) : bool :=
+    {
+      is_subtype sch (ListType lty) (ListType lty') := is_subtype sch lty lty';
 
-   Lemma subtypeP sch ty ty': reflect (Subtype sch ty ty') (is_subtype sch ty ty').
-   Proof.
-    apply: (iffP idP).
-    elim: ty ty' => n.
-      - case=>  //.
-        * by move=> n' /= /or3P [/eqP -> | Hi | Hu]; [apply ST_Refl | apply ST_Interface | apply ST_Union].
-        by move=> IH; case=> // => t' /= /IH; apply ST_ListType.
-    elim=> //=.
-      - elim=> //=.
-        * by move=> *; apply/or3P; constructor 1.
-      - by move=> * /=; apply/or3P; constructor 2.
-      by move=> * /=; apply/or3P; constructor 3.
-   Qed.
+      is_subtype sch (NT name) (NT name') :=
+        [|| (name == name'),
+         declares_implementation sch name name' | 
+         (name \in (union_members sch name'))];
+      
+      is_subtype _ _ _ := false
+    }.
+
+   (* Lemma subtypeP sch ty ty': reflect (Subtype sch ty ty') (is_subtype sch ty ty'). *)
+   (* Proof. *)
+   (*  apply: (iffP idP). *)
+   (*  elim: ty ty' => n. *)
+   (*    - case=>  //. *)
+   (*      * by move=> n' /= /or3P [/eqP -> | Hi | Hu]; [apply ST_Refl | apply ST_Interface | apply ST_Union]. *)
+   (*      by move=> IH; case=> // => t' /= /IH; apply ST_ListType. *)
+   (*  elim=> //=. *)
+   (*    - elim=> //=. *)
+   (*      * by move=> *; apply/or3P; constructor 1. *)
+   (*    - by move=> * /=; apply/or3P; constructor 2. *)
+   (*    by move=> * /=; apply/or3P; constructor 3. *)
+   (* Qed. *)
 
 
    (* Lemma is_subtype_is_same_or_in_possible_types sch (ty ty' : type) :
@@ -155,20 +158,17 @@ Section WellFormedness.
       by move=> t H /= /H; apply VList_Type.
   Qed.
 
-    Lemma obj_subtype sch (ty ty' : type) :
+    Lemma obj_subtypeE sch (ty ty' : type) :
      is_object_type sch ty ->
      is_subtype sch ty ty' ->
      [\/ ty' = ty,
       is_interface_type sch ty' |
       is_union_type sch ty'].
-   Proof.
-     move=> Hobj.
-     rewrite /is_subtype /=.
-     case: ty Hobj; case: ty' => // ty ty' Hobj.
-     move/or3P=> [/eqP -> | Hdecl | Hunion].
-       by constructor 1.
-       constructor 2. move/declares_in_implementation: Hdecl.
-   Abort.
+    Proof.
+      funelim (is_subtype sch ty ty') => //= Hobj.
+      - case/or3P => [/eqP -> | |]; first by constructor 1. 
+        * (* need conformance *)
+    Abort.
   
   (** 
       It checks whether an argument is well-formed by checking that
@@ -529,14 +529,7 @@ Section WellFormedness.
       by rewrite -Heq.
   Qed.
 
-  Lemma return_type_is_same_for_obj_and_supertype (schema : wfSchema) t ty :
-    t \in get_possible_types schema ty ->
-          forall f fld fld',
-            lookup_field_in_type schema t f = Some fld ->
-            lookup_field_in_type schema ty f = Some fld' ->
-            fld.(return_type) = fld'.(return_type).
-  Admitted.
-    
+ 
     
         
    Lemma field_in_interface_in_object_E (schema : wfSchema) ty ti f fld fld' :
@@ -646,9 +639,11 @@ Section WellFormedness.
      is_subtype schema (NT ty) (NT ty') ->
      ty = ty'.
    Proof.
-     move=> Hobj.
-     rewrite /is_subtype.
-     move/or3P=> [/eqP // | | ].
+     funelim (is_subtype schema (NT ty) (NT ty')) => //= Hobj.
+     case: H => ->.
+     case: H0 => ->.
+     case/or3P; first by apply/eqP.
+     
      move/declares_implementation_are_interfaces.
      by move: (is_object_type_interfaceN Hobj) => ->.
      move/in_union.
