src/QueryTactics.v
@@ -1,0 +1,65 @@
+
+From mathcomp Require Import all_ssreflect.
+Unset Printing Implicit Defensive.
+Set Asymmetric Patterns.
+
+From Equations Require Import Equations.
+
+Require Import SchemaAux.
+Require Import QueryAux.
+Require Import Ssromega.
+  
+  Ltac case_query q :=
+    repeat match goal with
+           | [H : context [q] |- _] => move: H
+           | [|- _] =>
+             let l := fresh "l" in
+             let f := fresh "f" in
+             let α := fresh "α" in
+             let β := fresh "β" in
+             let t := fresh "t" in
+             case: q => [f α | l f α | f α β | l f α β | t β]
+           end.
+    
+  
+  Ltac kill_neq :=
+    match goal with
+    | [H : ?x <> ?y |- context [_ != _]] => idtac "ok"
+    end.
+
+  
+  Ltac leq_queries_size :=
+    repeat match goal with
+           | [|- context [ query_size _]] => simp query_size => /=
+           | [|- context [ queries_size (_ ++ _)]] => rewrite queries_size_cat
+           | [|- context [ queries_size (merge_selection_sets (find_queries_with_label ?s ?rname ?ty ?qs)) ]] =>
+             let Hfleq := fresh in
+             let Hmleq := fresh in
+             have Hfleq := (found_queries_leq_size s rname ty qs);
+             have Hmleq := (merged_selections_leq (find_queries_with_label s rname ty qs)); ssromega                         
+     
+           | [|- context [queries_size (merge_selection_sets ?qs)]] =>
+              let Hfleq := fresh in
+              have Hfleq := (merged_selections_leq qs); ssromega                            
+         
+           | [|- context [queries_size (filter_queries_with_label ?rname ?qs)]] =>
+             let Hfleq := fresh in
+             have Hfleq := (filter_queries_with_label_leq_size rname qs); ssromega
+
+           | [|- context [queries_size (filter_queries_with_label ?rname1 ?qs1) +
+                         queries_size (filter_queries_with_label ?rname2 ?qs2)]] =>
+             let Hfleq1 := fresh in
+             let Hfleq2 := fresh in
+             have Hfleq1 := (filter_queries_with_label_leq_size rname1 qs1);
+             have Hfleq2 := (filter_queries_with_label_leq_size rname2 qs2); ssromega
+
+         
+           | [|- _] => ssromega
+    end.
+
+   Ltac lookup :=
+    match goal with
+    | [ |- context [ lookup_field_in_type _ _ _]] => let Hlook := fresh "Hlook" in
+                                                   let fld := fresh "fld" in
+                                                   case Hlook : lookup_field_in_type => //= [fld|]
+    end.
